\documentclass{article}
\usepackage[paperwidth=9cm,paperheight=9cm, margin=0.5cm]{geometry}
\usepackage{enumitem}
\pagenumbering{gobble}
\usepackage[ngerman,british]{babel}
\usepackage[utf8]{inputenc}
\usepackage[T1]{fontenc}
\usepackage{microtype}
\usepackage{lmodern}
\usepackage{amsthm}
\usepackage{amsmath}
\usepackage{amsfonts}
\usepackage{amssymb}
\usepackage{mathtools}
\usepackage{wasysym}
\usepackage{faktor}
\usepackage{tikz}


\begin{document}
\setlength{\parindent}{0pt}
%Problem hier
%Bei a), b), ... bitte dieses benutzen
%\begin{enumerate}[label=\alph*)]
%\end{enumerate}
Let $F=A_{0}A_{1}\dots A_{n}$ be a convex polygon in the plane. Define for all $1\le k\le n-1$ the operation $f_{k}$ which replaces $F$ with the new polygon$$f_{k}(F)=A_{0}\dots A_{k-1}A_{k}'A_{k+1}\dots A_{n},$$where $A_{k}'$ is the point symmetric to $A_{k}$ with respect to the perpendicular bisector of $A_{k-1}A_{k+1}$. Prove that $(f_{1}\circ f_{2}\circ\dots\circ f_{n-1})^{n}(F)=F$. We suppose that all operations are well-defined on the polygons, to which they are applied, i.e. results are convex polygons again. ($A_{0},A_{1},\dots,A_{n}$ are the vertices of $F$ in consecutive order.)
\end{document}
