\documentclass{article}
\usepackage[paperwidth=9cm,paperheight=9cm, margin=0.5cm]{geometry}
\usepackage{enumitem}
\pagenumbering{gobble}
\usepackage[ngerman,british]{babel}
\usepackage[utf8]{inputenc}
\usepackage[T1]{fontenc}
\usepackage{microtype}
\usepackage{lmodern}
\usepackage{amsthm}
\usepackage{amsmath}
\usepackage{amsfonts}
\usepackage{amssymb}
\usepackage{mathtools}
\usepackage{wasysym}
\usepackage{faktor}
\usepackage{tikz}


\begin{document}
\setlength{\parindent}{0pt}
%Problem hier
%Bei a), b), ... bitte dieses benutzen
%\begin{enumerate}[label=\alph*)]
%\end{enumerate}
For $n\ge0$ define matrices $A_{n}$ and $B_{n}$ as follows: $A_{0}=B_{0}=(1)$ and for every $n>0$$$A_{n}=\begin{pmatrix}A_{n-1}&A_{n-1}\\A_{n-1}&B_{n-1}\end{pmatrix}\text{ and }B_{n}=\begin{pmatrix}A_{n-1}&A_{n-1}\\A_{n-1}&0\end{pmatrix}.$$Denote the sum of all elements of a matrix $M$ by $S(M)$. Prove that $S(A_{n}^{k-1})=S(A^{n-1}_{k})$ for every $n,k\ge1$.
\end{document}
